src/lowparse/pulse/LowParse.PulseParse.BCVLI.fst
@@ -211,3 +211,45 @@ fn jump_bounded_bcvli
 }
 
 #pop-options
+
+(* leaf_reader for parse_bcvli *)
+
+#push-options "--z3rlimit 32 --z3cliopt smt.arith.nl=false --max_fuel 0"
+
+inline_for_extraction
+fn leaf_read_bcvli
+  (r1: PPB.leaf_reader (parse_bounded_integer_le 1))
+  (r2: PPB.leaf_reader (parse_bounded_integer_le 2))
+  (r4: PPB.leaf_reader (parse_bounded_integer_le 4))
+: PPB.leaf_reader parse_bcvli
+=
+  (input: S.slice byte)
+  (#pm: perm)
+  (#v: Ghost.erased U32.t)
+{
+  PPB.pts_to_parsed_elim input;
+  with w . assert (S.pts_to input #pm w);
+  parse_bcvli_eq w;
+  parser_kind_prop_equiv (parse_bounded_integer_kind 1) (parse_bounded_integer_le 1);
+  S.pts_to_len input;
+  let x = PPB.read_parsed_from_validator_success r1 input 0sz 1sz;
+  Seq.lemma_eq_elim
+    (Seq.slice w 1 (Seq.length w))
+    (Seq.slice w 1 (Seq.length w));
+  if (U32.lt x 253ul) {
+    Trade.elim _ _;
+    x
+  } else if (U32.eq x 253ul) {
+    parser_kind_prop_equiv (parse_bounded_integer_kind 2) (parse_bounded_integer_le 2);
+    let y = PPB.read_parsed_from_validator_success r2 input 1sz 3sz;
+    Trade.elim _ _;
+    y
+  } else {
+    parser_kind_prop_equiv (parse_bounded_integer_kind 4) (parse_bounded_integer_le 4);
+    let y = PPB.read_parsed_from_validator_success r4 input 1sz 5sz;
+    Trade.elim _ _;
+    y
+  }
+}
+
+#pop-options
